

João Paulo Nunes Andrade - 25002703

24/02/2020

1)
• f1)

$$F_1 = ((x_1 \cdot x_3) + (\overline{x_1} \cdot \overline{x_3})) \cdot ((x_2 \cdot x_4) + (\overline{x_2} \cdot \overline{x_4}))$$

▷ Porta XOR: $(A \cdot B) + (\bar{A} \cdot \bar{B}) = (A \oplus B)$

- Primeiro termo x_1 e x_3 : $(\overline{x_1 \oplus x_3})$
- Segundo termo x_2 e x_4 : $(\overline{x_2 \oplus x_4})$

$$\therefore F_1 = (\overline{x_1 \oplus x_3}) \cdot (\overline{x_2 \oplus x_4})$$

• f2)

$$\begin{aligned} F_2 &= (x_1 \cdot x_2 \cdot \bar{x}_3 \cdot \bar{x}_4) + (\bar{x}_1 \cdot \bar{x}_2 \cdot x_3 \cdot x_4) + (x_1 \cdot \bar{x}_2 \cdot \bar{x}_3 \cdot x_4) + (\bar{x}_1 \cdot x_2 \cdot x_3 \cdot \bar{x}_4) \\ &= x_1 \cdot \bar{x}_3 \cdot (\overline{x_2 \oplus x_4} + \overline{x_2 \oplus x_4}) + \bar{x}_1 \cdot \bar{x}_3 \cdot (\overline{x_2 \oplus x_4} + \overline{x_2 \oplus x_4}) \end{aligned}$$

\checkmark prova XOR: $(A \cdot \bar{B}) + (\bar{A} \cdot B) = (A \oplus B)$

$$\begin{aligned}
 \therefore f_2 &= x_1 \cdot \bar{x}_3 \cdot (x_2 \oplus x_4) + \bar{x}_1 \cdot x_3 \cdot (x_2 \oplus x_4) \\
 &= (x_1 \cdot \bar{x}_3 + \bar{x}_1 \cdot x_3) \cdot (x_2 \oplus x_4) \\
 &= (x_1 \oplus x_3) \cdot (x_2 \oplus x_4)
 \end{aligned}$$

Obs: f_1 não é equivalente a f_2

//
